Java/src/Semantics/SemCmdRules.v
@@ -48,15 +48,15 @@ Section Rules.
       (HPost : Q' |-- Q ) :
       {{P'}}c{{Q'}} |-- {{P}}c{{Q}}.
     Proof.
-      intros n Pr Hc Pr' m k s h HPr Hmn Hkm HP; simpl.
-      destruct (Hc _ _ _ s h HPr Hmn Hkm) as [HSafe HQ].
+      intros n Pr Hc Pr' m k s h t HPr Hmn Hkm HP; simpl.
+      destruct (Hc _ _ _ s h t HPr Hmn Hkm) as [HSafe HQ].
       + apply HPre; apply HP.
-      + split; [apply HSafe|intros h' s' H]. 
-        apply HPost. apply HQ. apply H.
+      + split; [apply HSafe|intros t' h' s' H]. 
+        apply HPost. apply HQ in H. apply H.
     Qed.
 
     Definition not_modifies (c : semCmd) (x : var) : Prop :=
-      forall PP s s' h h' n (HSem : c PP n s h (Some (s', h'))),
+      forall PP s s' h h' t t' n (HSem : c PP n s h t (Some (s', (h', t')))),
         s x = s' x.
 
     Lemma frame_rule : forall P Q R c (xs: list var)
@@ -65,21 +65,21 @@ Section Rules.
       {{ P ** R }} c {{ Q ** Exists vs, apply_subst R (subst_fresh vs xs) }}.
     Proof.
       intros.
-      intros ? PP HSpec PP' ? ? ? ? HPP' Hmn Hkm [h1 [h2 [HSub [HP HR]]]]; split.
+      intros ? PP HSpec PP' ? ? ? ? ? HPP' Hmn Hkm [h1 [h2 [HSub [HP HR]]]]; split.
       (* safety *)
-      { destruct (HSpec _ m k s h HPP' Hmn Hkm) as [HS _]; [ | assumption].
+      { destruct (HSpec _ m k s h t0 HPP' Hmn Hkm) as [HS _]; [ | assumption].
         solve_model HP. exists h2; apply HSub.
       }
       (* correctness *)
-      intros ? ? HSem. 
-      destruct (@cmd_frame c PP' s s' h h' h2 h1 k) as [h'' [HBig Hc]]. 
+      intros ? ? ? HSem. 
+      destruct (@cmd_frame c PP' s s' h h' h2 h1 k t0 t') as [h'' [HBig Hc]]. 
       + assumption.
-      + intros l Hle. destruct (HSpec _ m l s h1 HPP' Hmn) as [HS _];
+      + intros l Hle. destruct (HSpec _ m l s h1 t0 HPP' Hmn) as [HS _];
         assumption || omega.
       + assumption.
-      + destruct (HSpec _ m k s h1 HPP' Hmn Hkm) as [_ HC]. 
+      + destruct (HSpec _ m k s h1 t0 HPP' Hmn Hkm) as [_ HC]. 
         * apply HP.
-        * specialize (HC h'' s' Hc).
+        * specialize (HC t' h'' s' Hc).
           exists h'', h2, HBig. split. assumption.
           simpl. exists s. unfold apply_subst.
           solve_model HR.
@@ -95,7 +95,7 @@ Section Rules.
       G |-- {{P1 //\\ P2}} c {{Q1 //\\ Q2}}.
     Proof.
       intros n P HPP HG.
-      simpl. intros m k s h HPP' Hm Hk [HP1 HP2]. split.
+      simpl. intros m k s h t HPP' Hm Hk [HP1 HP2]. split.
       + eapply H1; eauto.
       + split; [eapply H1|eapply H2]; eauto.
     Qed.
@@ -106,73 +106,73 @@ Section Rules.
 
     Lemma skip_rule P : |-- {{P}}skip_cmd {{P}}.
     Proof.
-      intros n Pr HPP Pr' m k s h _ Hmn Hkm HP; split.
+      intros n Pr HPP Pr' m k s h t _ Hmn Hkm HP; split.
       + intro H; inversion H.
-      + intros h' s' HSem; inversion HSem; subst.
+      + intros t' h' s' HSem; inversion HSem; subst.
         solve_model HP.
     Qed.
 
     Lemma seq_rule c1 c2 P Q R :
       ({{P}}c1{{Q}} //\\ {{Q}}c2{{R}}) |-- {{P}}seq_cmd c1 c2{{R}}.
     Proof.
-      intros n Pr [Hc1 Hc2] Pr' k m s h HPP' Hmn Hkm HP; split.
+      intros n Pr [Hc1 Hc2] Pr' k m s h t HPP' Hmn Hkm HP; split.
       + intro HFail; inversion HFail; subst; clear HFail.
-        * destruct (Hc1 _ _ n0 s h HPP' Hmn) as [HS _];
+        * destruct (Hc1 _ _ n0 s h t HPP' Hmn) as [HS _];
           [omega | assumption | apply HS; exact H].
-        * destruct (Hc1 _ _ n0 s h HPP' Hmn) as [_ HC]; [omega | assumption |].
-          specialize (HC _ _ H).
-          destruct (Hc2 _ (k - n0) n' s' h' HPP') as [HS _]; [omega | omega | |].
+        * destruct (Hc1 _ _ n0 s h t HPP' Hmn) as [_ HC]; [omega | assumption |].
+          specialize (HC _ _ _ H).
+          destruct (Hc2 _ (k - n0) n' s' h' t' HPP') as [HS _]; [omega | omega | |].
           apply HC. apply HS. exact H0.
-      + intros h1 s1 HSem; inversion HSem; subst; clear HSem.
-        destruct (Hc1 _ _ n0 s h HPP' Hmn) as [_ HC1]; [omega | assumption |].
-        specialize (HC1 _ _ H5).
-        destruct (Hc2 _ (k - n0) n1 s2 h2 HPP') as [_ HC2]; [omega | omega | |].
-        apply HC1. specialize (HC2 _ _ H6).
+      + intros h1 s1 t1 HSem; inversion HSem; subst; clear HSem.
+        destruct (Hc1 _ _  n0 s h t HPP' Hmn) as [_ HC1]; [omega | assumption |].
+        specialize (HC1 _ _ _ H6).
+        destruct (Hc2 _ (k - n0) n1 s2 h2 t2 HPP') as [_ HC2]; [omega | omega | |].
+        apply HC1. specialize (HC2 _ _ _ H8).
         solve_model HC2.
     Qed.
 
     Lemma nondet_rule c1 c2 P Q :
       ({{P}}c1{{Q}} //\\ {{P}}c2{{Q}}) |-- {{P}}nondet_cmd c1 c2{{Q}}.
     Proof.
-      intros n Pr [Hc1 Hc2] Pr' k m s h HPP' Hmn Hkm HP; split.
+      intros n Pr [Hc1 Hc2] Pr' k m s h t HPP' Hmn Hkm HP; split.
       + intro HFail; inversion HFail; subst; clear HFail.
-        * destruct (Hc1 _ _ n0 s h HPP' Hmn) as [HS _];
+        * destruct (Hc1 _ _ n0 s h t HPP' Hmn) as [HS _];
           [omega | assumption | apply HS; exact H].
-        * destruct (Hc2 _ _ n0 s h HPP' Hmn) as [HS _];
+        * destruct (Hc2 _ _ n0 s h t HPP' Hmn) as [HS _];
           [omega | assumption | apply HS; exact H].
-      + intros h1 s1 HSem; inversion HSem; subst; clear HSem.
-        * destruct (Hc1 _ _ n0 s h HPP' Hmn) as [_ HC]; [omega | assumption |].
-          specialize (HC _ _ H4). solve_model HC.
-        * destruct (Hc2 _ _ n0 s h HPP' Hmn) as [_ HC]; [omega | assumption |].
-          specialize (HC _ _ H4). solve_model HC.
+      + intros h1 s1 t1 HSem; inversion HSem; subst; clear HSem.
+        * destruct (Hc1 _ _ n0 s h t HPP' Hmn) as [_ HC]; [omega | assumption |].
+          specialize (HC _ _ _ H5). solve_model HC.
+        * destruct (Hc2 _ _ n0 s h t HPP' Hmn) as [_ HC]; [omega | assumption |].
+          specialize (HC _ _ _ H5). solve_model HC.
     Qed.
 
     Lemma kleene_rule c P :
       {{P}}c{{P}} |-- {{P}} kleene_cmd c {{P}}.
     Proof.
-      intros n Pr Hc Pr' m k s h HPP' Hmn Hkm Hp; split.
+      intros n Pr Hc Pr' m k s h t HPP' Hmn Hkm Hp; split.
       + intro HFail. generalize dependent m. remember None as cfg.
         induction HFail; intros; inversion Heqcfg; subst.
-        * destruct (Hc _ m n0 s h HPP' Hmn) as [HS _];
+        * destruct (Hc _ m n0 s h t HPP' Hmn) as [HS _];
           [omega | assumption | apply HS; exact H].
-        * destruct (Hc _ m n0 s h HPP' Hmn) as [_ HC]; [omega | assumption |].
+        * destruct (Hc _ m n0 s h t HPP' Hmn) as [_ HC]; [omega | assumption |].
           apply IHHFail with (m-n0); [assumption | reflexivity | omega | omega | ].
-          specialize (HC _ _ H). solve_model HC.
-      + intros. remember (Some (s', h')) as cfg. generalize dependent m. 
+          specialize (HC _ _ _ H). solve_model HC.
+      + intros. remember (Some (s', (h', t'))) as cfg. generalize dependent m. 
         induction H; inversion Heqcfg; subst; intros.
         * solve_model Hp.
-        * destruct (Hc _ m n0 s h HPP' Hmn) as [_ HC]; [omega | assumption |].
+        * destruct (Hc _ m n0 s h t HPP' Hmn) as [_ HC]; [omega | assumption |].
           assert ((((P s') P0) ((m - n0) - n1)) h') as H1. 
-          apply IHkleene_sem; try assumption; try omega. apply HC; assumption.
+          apply IHkleene_sem; try assumption; try omega. apply HC in H; assumption.
           solve_model H1.
     Qed.
 
     Lemma assume_rule P (t : vlogic) :
       |-- {{P}} assume_cmd t {{t /\\ P}}.
     Proof.
-      intros n Pr Hc Pr' m k s h HPP' Hmn Hkm Hp; split.
+      intros n Pr Hc Pr' m k s h tr HPP' Hmn Hkm Hp; split.
       + intros HFail. inversion HFail.
-      + intros h' s' H. remember (Some (s', h')) as cfg; induction H.
+      + intros tr' h' s' H. remember (Some (s', (h', tr'))) as cfg; induction H.
         inversion Heqcfg; subst; intros.
         split; [assumption|]. solve_model Hp.
     Qed.
@@ -180,9 +180,9 @@ Section Rules.
     Lemma assert_rule (P : sasn) (p : vlogic) (HPe : P |-- embed p) :
       |-- {{P}} assert_cmd p {{P}}.
     Proof.
-      intros n Pr Hc Pr' m k s h HPP' Hmn Hkm Hp; specialize (HPe _ _ _ _ Hp); split.
+      intros n Pr Hc Pr' m k s h t HPP' Hmn Hkm Hp; specialize (HPe _ _ _ _ Hp); split.
       + intro HF; inversion HF; subst; auto.
-      + intros h' s' HSem; inversion HSem; subst. solve_model Hp.
+      + intros t' h' s' HSem; inversion HSem; subst. solve_model Hp.
     Qed.
 
   End PrimitivesRules.
@@ -191,8 +191,8 @@ Section Rules.
     (Forall x, {{P x}} c {{q}}) -|- {{Exists x, P x}} c {{q}}.
   Proof.
   	split.
-  	+ intros n Pr Hp Pr' m k s h HPP' Hmn Hkm [x Hxp]; specialize (Hp x); auto.
-  	+ intros n Pr Hp x Pr' m k s h HPP' Hmn Hkm Hxp.
+  	+ intros n Pr Hp Pr' m k s h t HPP' Hmn Hkm [x Hxp]; specialize (Hp x); auto.
+  	+ intros n Pr Hp x Pr' m k s h t HPP' Hmn Hkm Hxp.
   	  apply Hp; try assumption. exists x; apply Hxp.
   Qed.
 
@@ -202,10 +202,10 @@ Section Rules.
     (SP -->> {{ P }} c {{ Q }}) -|- {{ SP /\\  P }} c {{ Q }}.
   Proof.
   	split.
-  	+ intros Pr n Hp Pr' m k s h HPP' Hmn Hkm [HSP HP].
+  	+ intros Pr n Hp Pr' m k s h t HPP' Hmn Hkm [HSP HP].
   	  specialize (Hp Pr' HPP' m Hmn HSP).
   	  apply Hp; reflexivity || assumption.
-  	+ intros Pr n Hp Pr' HPP' m Hnm HSP Pr'' k l s h HPP'' Hkm Hkl HP.
+  	+ intros Pr n Hp Pr' HPP' m Hnm HSP Pr'' k l s h t HPP'' Hkm Hkl HP.
   	  apply Hp.
   	  * transitivity Pr'; assumption.
   	  * omega.
